\section{Conic Sections}

\begin{mydef}
A \emph{Conic} in $\mathbb{R}^2$ is a plane curve given by the quadratic
equation
\[
q(x,y) = ax^2 + bxy + cy^2 + dx + ey + f = 0
\]
\end{mydef}

To ``adapt" this definition into projective space $\mathbb{P}^2$, we simply
note that the inhomogenous polynomial $q$ has an associated
homogenous polynomial 
\[
Q(X,Y,Z) = aX^2 + bXY + cY^2 + dXZ + eYZ + fZ^2
\]
Miles Reid recommends thinking about this as a bijection $q \leftrightarrow Q$ by
\[
q(x,y) = Q(\frac{X}{Z},\frac{Y}{Z},\frac{Z}{Z}),~Z\ne 0
\]
Thus, a conic in $\mathbb{P}^2$ would be determined by the zeroes of $Q$.

\begin{theorem}
Let $k$ be any field of characteristic $\ne 2$. Then, any quadratic form $Q$
in $(X,Y,Z)$ has an associated $3 \times 3$ symmetric matrix $A$ s.t.
\[
x^TAx =  Q(X,Y,Z),~x=\begin{bmatrix}
x\\
y\\
z
\end{bmatrix}
\]
explicitly, if 
\[
Q(X,Y,Z) = aX^2 + 2bXY + cY^2 + 2dXZ + 2eYZ + fZ^2
\]
Then
\[
A = \begin{bmatrix}
a & b & d\\
b & c & e\\
d & e & f
\end{bmatrix}
\]
and the quadratic form (and hence the conic it defines) is non-degenerate
if the matrix $A$ is non-degenerate (non-singular).
\end{theorem}

Note that the matrix $A$ from the above theorem is symmetric. Thus, we can
apply the Spectral Theorem to see that we can diagonalize it using some
orthogonal matrix. This effectively allows us to transform any non-degenerate 
quadratic form into a homogenous quadratic form through a change of basis.

\begin{theorem}
Let $Q$ be a quadratic form of $X, Y, Z$. Then, there exists a change of basis $(X,Y,Z) \mapsto (X',Y',Z')$ s.t.
$Q(X,Y,Z) = Q'(X',Y',Z')$ where
\[
Q'(X',Y',Z') = \lambda_1 X'^2 + \lambda_2 Y'^2 + \lambda_3 Z'^2
\]
As a corollary, all non-degenerate conics in $\mathbb{P}^2$ are projectively
equivalent to the conic defined by $XZ = Y^2$. That is, there is some
projective transformation which takes an arbitrary conic $C$ to the conic 
defined by $XZ = Y^2$.
\end{theorem}
\begin{proof}
$Q$ is a quadratic form,
thus $Q$ has an associated symmetric matrix 
$A$ s.t. $Q(x) = x^TAx$. As $A$ is symmetric, the Spectral Theorem gives that
\[
\exists P:~P\text{ orthogonal},~P^TAP\text{ is diagonal}
\]
and in fact, the diagonal entries of $B=P^TAP$ are the eigenvalues of $A$. Thus,
it is easy to show, using the transformation $x=Px'$, that
\[
Q(X,Y,Z) = x^TAx = (Px')^TAPx' = x'^TP^TAPx' = x'^TBx'
\]
Now, letting the eigenvalues of $A$ be $\lambda_1, \lambda_2, \lambda_3$ we see that
\[
x'^TBx' = \lambda_1 X'^2 + \lambda_2 Y'^2 + \lambda_3 Z'^2 = Q'(X',Y',Z')
\]
Thus, $Q(X,Y,Z) = Q'(X',Y',Z')$.
\end{proof}
